lib/Crypto.lean
@@ -1,1 +1,4 @@
 import Crypto.Mceliece.Ref348864
+import Crypto.Prim.AES
+import Crypto.Prim.Shake
+import Crypto.Random.DRBG
