lib/Crypto/Prim/AES.lean
@@ -1,0 +1,4 @@
+import Crypto.ByteVec
+
+@[extern "lean_AES256_ECB"]
+opaque aes256Ecb (key: @&ByteVec 32) (v: @&ByteVec 16) : ByteVec 16
