lib/Crypto/Random/DRBG.lean
@@ -1,0 +1,88 @@
+import Crypto.Prim.AES
+import Crypto.Random.PRNG
+import Crypto.Nat
+import Crypto.Range
+import Crypto.Vector
+
+-- theorem mul_div_lt {i m n:Nat} : i < m * n → (i/n) < m := by admit
+
+def concatByteVec (v : Vector m (ByteVec n)) : ByteVec (m*n) :=
+  let r {i} (p : i < m*n) : 0 < n := sorry
+  ByteVec.generate (m*n) (λi => (v.get ⟨i.val / n, Nat.mul_div_lt i.isLt⟩).get (Fin.ofNat' i.val (r i.isLt)))
+
+structure DRBG where
+  key : ByteVec (256 / 8)
+  v : ByteVec (128 / 8)
+
+instance : Inhabited DRBG := ⟨Inhabited.default, Inhabited.default⟩
+
+@[reducible]
+def Seed := ByteVec 48
+
+opaque incrementV (v : ByteVec 16) : ByteVec 16 := Id.run do
+  let mut v := v
+  for i in range 0 15 do
+    let j := 15 - i
+    let vj := v.get! j
+    if vj = 0xff then
+      v := v.set! j 0x00
+    else
+      v := v.add! j 1
+      break
+  pure v
+
+opaque aes256CtrDrbgUpdate (key : ByteVec 32) (v0 : ByteVec 16) : ByteVec 48 :=
+  let g := Vector.iterate 3 incrementV (incrementV v0)
+  concatByteVec (aes256Ecb key <$> g)
+
+opaque randombytesInit (s : Seed) : DRBG :=
+  let key := ByteVec.generate 32 (λ_ => 0)
+  let v   := ByteVec.generate 16 (λ_ => 0)
+  let b := aes256CtrDrbgUpdate key v
+  let b := ByteVec.generate _ (λi => b.get i ^^^ s.get i)
+  { key := b.extractN 0 32, v := b.extractN 32 16 }
+
+private theorem randomBytesTerminates : ∀ n, n ≥ 16 → n - 16 < n := by
+  intros n gt
+  have n_pos : 0 < n := by
+        cases n with
+        | zero =>
+          contradiction
+        | succ x =>
+          exact (Nat.zero_lt_succ _)
+  apply Nat.sub_lt n_pos (by decide)
+
+def randombytes3 (key : ByteVec 32) (v : ByteVec 16) (a : ByteArray) (n : Nat)
+   : ByteArray × ByteVec 16 :=
+  if n == 0 then
+    (a, v)
+  else
+    let v := incrementV v
+    let b := aes256Ecb key v
+    if h : n ≥ 16 then
+      have : n - 16 < n := randomBytesTerminates n ‹_›
+      randombytes3 key v (a ++ b.data) (n - 16)
+    else
+      (a ++ b.data.extractN 0 n, v)
+
+--theorem randomBytes3_size2 (key) (v) (a) (n:Nat)
+--    : (randombytes3 key v a n).1.size = a.size + n := by admit
+
+theorem randomBytes3_size (key) (v) (a) (n:Nat)
+    : (randombytes3 key v a n).1.size = n := by
+  admit
+
+namespace DRBG
+
+opaque randombytes (rbg : DRBG) (n : Nat) : ByteVec n × DRBG :=
+  let key := rbg.key
+  let v := rbg.v
+  let p := randombytes3 key v (ByteArray.mkEmpty n) n
+  let pr : p.1.size = n := randomBytes3_size key v (ByteArray.mkEmpty n) n
+  let b := aes256CtrDrbgUpdate key p.2
+  let rbg := { key := b.extractN 0 32, v := b.extractN 32 16 }
+  (⟨p.1, pr⟩, rbg)
+
+instance : PRNG DRBG := ⟨DRBG.randombytes⟩
+
+end DRBG
